

3. Multivariate linear regression is widely used to model the relationships between multiple related responses and a set of predictors. Suppose we have N observations of m -dimensional responses $Y_i = (y_{i,1}, \dots, y_{i,m})^\top$ and p -dimensional predictors $X_i = (x_{i,1}, \dots, x_{i,p})^\top$, for $i = 1, \dots, N$. Let $\mathbf{Y} = (Y_1, \dots, Y_N)^\top$ be the $N \times m$ response matrix and $\mathbf{X} = (X_1, \dots, X_N)^\top$ be the $N \times p$ covariates matrix. The multivariate linear regression model assumes

$$\mathbf{Y} = \mathbf{X}B + E,$$

where B is a $p \times m$ matrix of unknown regression parameters and $E = (\epsilon_1, \dots, \epsilon_N)^\top$ is an $N \times m$ matrix of regression errors, with ϵ_i 's independently sampled from an m -dimensional Gaussian distribution $N(\mathbf{0}, \Sigma)$.

- (a) For the multivariate linear regression model, derive the Maximum Likelihood Estimator (MLE) of B and Σ .
- (b) Similarly to the unidimensional linear regression model, the Ordinary Least Squares (OLS) estimator of B is defined as the minimizer of the Residual Sum of Squares (RSS) defined as

$$RSS(B) = \sum_{i=1}^N (Y_i^\top - X_i^\top B)(Y_i^\top - X_i^\top B)^\top.$$

Derive the OLS estimator of B . Is it the same as the MLE?

$$(a) L(B, \Sigma) = \prod_{i=1}^N \frac{1}{(2\pi)^{\frac{m}{2}} |\Sigma|^{\frac{1}{2}}} \exp\left(-\frac{1}{2} (Y_i - B^\top X_i)^\top \Sigma^{-1} (Y_i - B^\top X_i)\right) \quad \text{--- likelihood function}$$

$$l(B, \Sigma) = \ln(B, \Sigma) = -\frac{Nm}{2} \ln(2\pi) - \frac{N}{2} \ln |\Sigma| - \frac{1}{2} \sum_{i=1}^N (Y_i - B^\top X_i)^\top \Sigma^{-1} (Y_i - B^\top X_i)$$

$$\text{here } \sum_{i=1}^N (Y_i - B^\top X_i)^\top \Sigma^{-1} (Y_i - B^\top X_i) = \text{tr}(\Sigma^{-1} (Y - XB)^\top (Y - XB)) \Rightarrow l(B, \Sigma) = C - \frac{N}{2} \ln |\Sigma| - \frac{1}{2} \text{tr}(\Sigma^{-1} (Y - XB)^\top (Y - XB))$$

$$\text{according to } \frac{\partial}{\partial B} \text{tr}(\Sigma^{-1} (Y - XB)^\top (Y - XB)) = -2X^\top (Y - XB) \Sigma^{-1}, \text{ let } -2X^\top (Y - XB) \Sigma^{-1} = 0 \Rightarrow X^\top Y = X^\top X B$$

$$\Rightarrow \hat{B}_{MLE} = (X^\top X)^{-1} X^\top Y$$

$$\text{define } S := (Y - XB)^\top (Y - XB) \Rightarrow l(\Sigma) = -\frac{N}{2} \ln |\Sigma| - \frac{1}{2} \text{tr}(\Sigma^{-1} S)$$

$$\text{Here } \frac{\partial l}{\partial \Sigma^{-1}} = \frac{N}{2} \Sigma - \frac{1}{2} S = 0 \Rightarrow \hat{\Sigma}_{MLE} = \frac{1}{N} S = \frac{1}{N} (Y - X \hat{B}_{MLE})^\top (Y - X \hat{B}_{MLE})$$

$$(b) RSS(B) = \text{tr}((Y - XB)^\top (Y - XB)) = \text{tr}(Y^\top Y - Y^\top X B - B^\top X^\top Y + B^\top X^\top X B)$$

$$\frac{\partial RSS}{\partial B} = \frac{\partial}{\partial B} \text{tr}(-2Y^\top X B + B^\top X^\top X B) = -2X^\top Y + 2X^\top X B, \text{ let } \frac{\partial RSS}{\partial B} = 0 \Rightarrow X^\top X B = X^\top Y \Rightarrow \hat{B}_{OLS} = (X^\top X)^{-1} X^\top Y$$

$$\hat{B}_{OLS} = \hat{B}_{MLE}$$